SR partly working, SL needs fixing

SP1Chips/ShiftLeft/Constraints.lean
@@ -4,10 +4,12 @@ import SP1Operations.Reader.ALUTypeReader
 
 namespace ShiftLeft
 
+variable (Main : Vector (Fin BB) 65)
+
 section constraints
 
 -- Generated Lean code for chip ShiftLeftChip
-def constraints (Main : Vector (Fin BB) 65) : SP1ConstraintList :=
+def constraints  : SP1ConstraintList :=
   let E0 : Fin BB := Main[62] + Main[63]
   let E1 : Fin BB := E0 - 1
   let E2 : Fin BB := E0 * E1
@@ -343,7 +345,7 @@ lemma allHold_constraints_iff :
 
 end constraints
 
-section field
+section field_arithmetic
 
 lemma cancel_mul_65536 { a b c x : Fin BB } (h_dvd : (x : ℕ) ∣ 65536) : a * x = b * 65536 + c * x → a = b * ((65536 : ℕ) / (x : ℕ)) + c
   := by
@@ -383,113 +385,26 @@ lemma is_mod_64 {c0 m : Fin BB} : m < 64 → c0 < 65536 → ((c0 - m) * 19818086
         assumption
       . omega
 
-end field
+end field_arithmetic
+
+section opcode_defs
+
+@[simp] def is_sll := Main[62] = 1 ∧ Main[31] = 0
+@[simp] def is_sllw := Main[63] = 1 ∧ Main[31] = 0
+@[simp] def is_slli := Main[62] = 1 ∧ Main[31] = 1
+@[simp] def is_slliw := Main[63] = 1 ∧ Main[31] = 1
+
+end opcode_defs
 
 section sll
-
-@[simp] def is_sll (Main : Vector (Fin BB) 65) := Main[62] = 1 ∧ Main[31] = 0
-
-set_option maxHeartbeats 1000000 in
-lemma allHold_constraints_iff_sll (h : is_sll Main) :
-  List.Forall SP1Constraint.toProp (constraints Main) ↔
-    List.Forall SP1Constraint.toProp (U16MSBOperation.constraints Main[33] { msb := Main[61] } 0) ∧
-    List.Forall SP1Constraint.toProp (CPUState.constraints { clk_high := Main[0], clk_16_24 := Main[1], clk_0_16 := Main[2], pc := #v[Main[3], Main[4], Main[5]] } #v[Main[3] + 4, Main[4], Main[5]] 8 1) ∧
-    List.Forall SP1Constraint.toProp (ALUTypeReader.constraints Main[0] (Main[2] + Main[1] * 65536) #v[Main[3], Main[4], Main[5]] 6 #v[Main[64], 1, 0] #v[Main[32], Main[33], Main[34], Main[35]] { op_a := Main[6], op_a_memory := { prev_value := #v[Main[7], Main[8], Main[9], Main[10]], access_timestamp := { prev_low := Main[11], diff_low_limb := Main[12] } }, op_a_0 := Main[13], op_b := Main[14], op_b_memory := { prev_value := #v[Main[15], Main[16], Main[17], Main[18]], access_timestamp := { prev_low := Main[19], diff_low_limb := Main[20] } }, op_c := #v[Main[21], Main[22], Main[23], Main[24]], op_c_memory := { prev_value := #v[Main[25], Main[26], Main[27], Main[28]], access_timestamp := { prev_low := Main[29], diff_low_limb := Main[30] } }, imm_c := 0 } 1) ∧
-    (Main[36] = 0 ∨ Main[36] = 1) ∧
-    (Main[37] = 0 ∨ Main[37] = 1) ∧
-    (Main[38] = 0 ∨ Main[38] = 1) ∧
-    (Main[39] = 0 ∨ Main[39] = 1) ∧
-    (Main[40] = 0 ∨ Main[40] = 1) ∧
-    (Main[41] = 0 ∨ Main[41] = 1) ∧
-    (((Main[25] - (Main[36] + Main[37] * 2 + Main[38] * 4 + Main[39] * 8 + Main[40] * 16 + Main[41] * 32)) * 1981808641).val < 1024) ∧
-    (Main[45] = 0 ∨ Main[40] + Main[41] * 2 * 1 = 0) ∧
-    (Main[45] = 0 ∨ Main[45] = 1) ∧
-    (Main[46] = 0 ∨ Main[40] + Main[41] * 2 * 1 = 1) ∧
-    (Main[46] = 0 ∨ Main[46] = 1) ∧
-    (Main[47] = 0 ∨ Main[40] + Main[41] * 2 * 1 = 2) ∧
-    (Main[47] = 0 ∨ Main[47] = 1) ∧
-    (Main[48] = 0 ∨ Main[40] + Main[41] * 2 * 1 = 3) ∧
-    (Main[48] = 0 ∨ Main[48] = 1) ∧
-    (Main[45] + Main[46] + Main[47] + Main[48] = 1) ∧
-    (Main[42] = (Main[36] + 1) * (Main[37] * 3 + 1)) ∧
-    (Main[43] = Main[42] * (Main[38] * 15 + 1)) ∧
-    (Main[44] = Main[43] * (Main[39] * 255 + 1)) ∧
-    (Main[49].val < 2 ^ ((16 : Fin BB) - (Main[36] + Main[37] * 2 + Main[38] * 4 + Main[39] * 8)).val) ∧
-    (Main[53].val < 2 ^ (Main[36] + Main[37] * 2 + Main[38] * 4 + Main[39] * 8).val) ∧
-    (Main[15] * Main[44] = Main[53] * 65536 + Main[49] * Main[44]) ∧
-    (Main[50].val < 2 ^ ((16 : Fin BB) - (Main[36] + Main[37] * 2 + Main[38] * 4 + Main[39] * 8)).val) ∧
-    (Main[54].val < 2 ^ (Main[36] + Main[37] * 2 + Main[38] * 4 + Main[39] * 8).val) ∧
-    (Main[16] * Main[44] = Main[54] * 65536 + Main[50] * Main[44]) ∧
-    (Main[51].val < 2 ^ ((16 : Fin BB) - (Main[36] + Main[37] * 2 + Main[38] * 4 + Main[39] * 8)).val) ∧
-    (Main[55].val < 2 ^ (Main[36] + Main[37] * 2 + Main[38] * 4 + Main[39] * 8).val) ∧
-    (Main[17] * Main[44] = Main[55] * 65536 + Main[51] * Main[44]) ∧
-    (Main[52].val < 2 ^ ((16 : Fin BB) - (Main[36] + Main[37] * 2 + Main[38] * 4 + Main[39] * 8)).val) ∧
-    (Main[56].val < 2 ^ (Main[36] + Main[37] * 2 + Main[38] * 4 + Main[39] * 8).val) ∧
-    (Main[18] * Main[44] = Main[56] * 65536 + Main[52] * Main[44]) ∧
-    (Main[57] = Main[49] * Main[44]) ∧
-    (Main[58] = Main[50] * Main[44] + Main[53]) ∧
-    (Main[59] = Main[51] * Main[44] + Main[54]) ∧
-    (Main[60] = Main[52] * Main[44] + Main[55]) ∧
-    (Main[45] = 0 ∨ Main[32] = Main[57]) ∧
-    (Main[45] = 0 ∨ Main[33] = Main[58]) ∧
-    (Main[45] = 0 ∨ Main[34] = Main[59]) ∧
-    (Main[45] = 0 ∨ Main[35] = Main[60]) ∧
-    (Main[46] = 0 ∨ Main[32] = 0) ∧
-    (Main[46] = 0 ∨ Main[33] = Main[57]) ∧
-    (Main[46] = 0 ∨ Main[34] = Main[58]) ∧
-    (Main[46] = 0 ∨ Main[35] = Main[59]) ∧
-    (Main[47] = 0 ∨ Main[32] = 0) ∧
-    (Main[47] = 0 ∨ Main[33] = 0) ∧
-    (Main[47] = 0 ∨ Main[34] = Main[57]) ∧
-    (Main[47] = 0 ∨ Main[35] = Main[58]) ∧
-    (Main[48] = 0 ∨ Main[32] = 0) ∧
-    (Main[48] = 0 ∨ Main[33] = 0) ∧
-    (Main[48] = 0 ∨ Main[34] = 0) ∧
-    (Main[48] = 0 ∨ Main[35] = Main[57]) ∧
-    (Main[63] = 0) ∧
-    (Main[64] = 51)
-   := by
-  obtain ⟨ m62, m31 ⟩ := h
-  simp_all [allHold_constraints_iff, constraints, sub_eq_zero]
-  constructor <;> intro cstrs
-  . obtain ⟨ msb, cpu, alu,
-             b_m62, b_m63,
-             b_m36, b_m37, b_m38, b_m39, b_m40, b_m41,
-             diff_m25,
-             eq_m45, b_m45, eq_m46, b_m46, eq_m47, b_m47, eq_m48, b_m48,
-             one_of_45_46_47_48,
-             eq_m42, eq_m43, eq_m44,
-             lt_m49, lt_m53, h_15_44,
-             lt_m50, lt_m54, h_16_44,
-             lt_m51, lt_m55, h_17_44,
-             lt_m52, lt_m56, h_18_44,
-             eq_m57, eq_m58, eq_m59, eq_m60,
-             sll_00, sll_01, sll_02, sll_03, sll_04, sll_05, sll_06, sll_07, sll_08, sll_09, sll_10, sll_11, sll_12, sll_13, sll_14, sll_15,
-             sllw_00, sllw_01, sllw_02, sllw_03, sllw_04, sllw_05,
-             eq_m64 ⟩ := cstrs
-    have : Main[63] = 0 := by clear *- b_m62 b_m63; aesop
-    simp_all
-  . obtain ⟨ msb, cpu, alu,
-             b_m36, b_m37, b_m38, b_m39, b_m40, b_m41,
-             diff_m25,
-             eq_m45, b_m45, eq_m46, b_m46, eq_m47, b_m47, eq_m48, b_m48,
-             one_of_45_46_47_48,
-             eq_m42, eq_m43, eq_m44,
-             lt_m49, lt_m53, h_15_44,
-             lt_m50, lt_m54, h_16_44,
-             lt_m51, lt_m55, h_17_44,
-             lt_m52, lt_m56, h_18_44,
-             eq_m57, eq_m58, eq_m59, eq_m60,
-             sll_00, sll_01, sll_02, sll_03, sll_04, sll_05, sll_06, sll_07, sll_08, sll_09, sll_10, sll_11, sll_12, sll_13, sll_14, sll_15,
-             eq_m63, eq_m64 ⟩ := cstrs
-    simp_all
 
 set_option maxHeartbeats 100000000 in
 lemma spec.sll (h : is_sll Main) :
   List.Forall SP1Constraint.toProp (constraints Main) →
     Word.toBitVec64 #v[Main[32], Main[33], Main[34], Main[35]] = execute_RTYPE_pure_w #v[Main[15], Main[16], Main[17], Main[18]] #v[Main[25], Main[26], Main[27], Main[28]] .SLL
   := by sorry
-    -- intro cstrs; rw [allHold_constraints_iff_sll h] at cstrs
+    -- intro cstrs; rw [allHold_constraints_iff] at cstrs
+    -- obtain ⟨ eq_sll, eq_imm ⟩ := h
 
     -- set b0 := Main[15]
     -- set b1 := Main[16]
@@ -499,6 +414,7 @@ lemma spec.sll (h : is_sll Main) :
     -- set c1 := Main[26]
     -- set c2 := Main[27]
     -- set c3 := Main[28]
+    -- set imm := Main[31]
     -- set a0 := Main[32]
     -- set a1 := Main[33]
     -- set a2 := Main[34]
@@ -529,25 +445,31 @@ lemma spec.sll (h : is_sll Main) :
     -- set lr2 := Main[59]
     -- set lr3 := Main[60]
     -- set msb := Main[61]
+    -- set sll := Main[62]
+    -- set sllw := Main[63]
 
-    -- obtain ⟨ eq_m62, eq_m31 ⟩ := h
-    -- obtain ⟨ msb_cstrs, cpu_cstrs, alu_cstrs,
-    --          b_cb0, b_cb1, b_cb2, b_cb3, b_cb4, b_cb5,
-    --          diff,
-    --          eq_su160, b_su160, eq_su161, b_su161, eq_su162, b_su162, eq_su163, b_su163,
-    --          one_of_su16,
+    -- obtain ⟨ msb_a1, cpu, alu, one_of_ops,
+    --          b_sll, b_sllw,
+    --          b_cb0, b_cb1, b_cb2, b_cb3, b_cb4, b_cb5, diff,
+    --          h_su160, b_su160, h_su161, b_su161, h_su162, b_su162, h_su163, b_su163, one_of_su16s,
     --          eq_v01, eq_v012, eq_v0123,
-    --          lt_ll0, lt_hl0, h_b0_dec,
-    --          lt_ll1, lt_hl1, h_b1_dec,
-    --          lt_ll2, lt_hl2, h_b2_dec,
-    --          lt_ll3, lt_hl3, h_b3_dec,
+    --          lt_ll0, lt_lh0, h_b0_dec, lt_ll1, lt_lh1, h_b1_dec,
+    --          lt_ll2, lt_lh2, h_b2_dec, lt_ll3, lt_lh3, h_b3_dec,
     --          eq_lr0, eq_lr1, eq_lr2, eq_lr3,
-    --          sll_00, sll_01, sll_02, sll_03, sll_04, sll_05, sll_06, sll_07, sll_08, sll_09, sll_10, sll_11, sll_12, sll_13, sll_14, sll_15,
-    --          eq_m63, eq_m64 ⟩ := cstrs
-    -- clear msb_cstrs cpu_cstrs
-    -- rw [ALUTypeReader.allHold_constraints_iff_is_real (by rfl)] at alu_cstrs
-    -- simp [Opcode.ofNat, Nat.ble, Nat.beq] at alu_cstrs
-    -- obtain ⟨ h0, h1, h2, h3, h4, h5, h6, h7, h8, h9, h10, h11, h12, h13, h14, is_U64_b, ⟨ h15, h16, is_U64_c ⟩, h17 ⟩ := alu_cstrs
+    --          nw_00, nw_01, nw_02, nw_03, nw_04, nw_05, nw_06, nw_07, nw_08, nw_09, nw_10, nw_11, nw_12, nw_13, nw_14, nw_15,
+    --          w_00, w_01, w_02, w_03, w_04, w_05,
+    --          eq_m64 ⟩ := cstrs
+
+    -- have eq_m63 : sllw = 0 := by
+    --   clear *- b_sll b_sllw one_of_ops eq_sll
+    --   simp_all; aesop
+
+    -- simp_all
+
+    -- clear msb_a1 cpu
+    -- rw [ALUTypeReader.allHold_constraints_iff_is_real (by rfl)] at alu
+    -- simp [Opcode.ofNat, Nat.ble, Nat.beq] at alu
+    -- obtain ⟨ h0, h1, h2, h3, h4, h5, h6, h7, h8, h9, h10, h11, h12, h13, h14, is_U64_b, ⟨ h15, h16, is_U64_c ⟩, h17 ⟩ := alu
     -- clear h0 h1 h2 h3 h4 h5 h6 h7 h8 h9 h10 h11 h12 h13 h14 h15 h16 h17
     -- simp_all
 
@@ -599,322 +521,14 @@ end sll
 
 section slli
 
-@[simp] def is_slli (Main : Vector (Fin BB) 65) := Main[62] = 1 ∧ Main[31] = 1
-
-set_option maxHeartbeats 1000000 in
-lemma allHold_constraints_iff_slli (h : is_slli Main) :
-  List.Forall SP1Constraint.toProp (constraints Main) ↔
-    List.Forall SP1Constraint.toProp (U16MSBOperation.constraints Main[33] { msb := Main[61] } 0) ∧
-    List.Forall SP1Constraint.toProp (CPUState.constraints { clk_high := Main[0], clk_16_24 := Main[1], clk_0_16 := Main[2], pc := #v[Main[3], Main[4], Main[5]] } #v[Main[3] + 4, Main[4], Main[5]] 8 1) ∧
-    List.Forall SP1Constraint.toProp (ALUTypeReader.constraints Main[0] (Main[2] + Main[1] * 65536) #v[Main[3], Main[4], Main[5]] 6 #v[Main[64], 1, 0] #v[Main[32], Main[33], Main[34], Main[35]] { op_a := Main[6], op_a_memory := { prev_value := #v[Main[7], Main[8], Main[9], Main[10]], access_timestamp := { prev_low := Main[11], diff_low_limb := Main[12] } }, op_a_0 := Main[13], op_b := Main[14], op_b_memory := { prev_value := #v[Main[15], Main[16], Main[17], Main[18]], access_timestamp := { prev_low := Main[19], diff_low_limb := Main[20] } }, op_c := #v[Main[21], Main[22], Main[23], Main[24]], op_c_memory := { prev_value := #v[Main[25], Main[26], Main[27], Main[28]], access_timestamp := { prev_low := Main[29], diff_low_limb := Main[30] } }, imm_c := 1 } 1) ∧
-    (Main[36] = 0 ∨ Main[36] = 1) ∧
-    (Main[37] = 0 ∨ Main[37] = 1) ∧
-    (Main[38] = 0 ∨ Main[38] = 1) ∧
-    (Main[39] = 0 ∨ Main[39] = 1) ∧
-    (Main[40] = 0 ∨ Main[40] = 1) ∧
-    (Main[41] = 0 ∨ Main[41] = 1) ∧
-    (((Main[25] - (Main[36] + Main[37] * 2 + Main[38] * 4 + Main[39] * 8 + Main[40] * 16 + Main[41] * 32)) * 1981808641).val < 1024) ∧
-    (Main[45] = 0 ∨ Main[40] + Main[41] * 2 * 1 = 0) ∧
-    (Main[45] = 0 ∨ Main[45] = 1) ∧
-    (Main[46] = 0 ∨ Main[40] + Main[41] * 2 * 1 = 1) ∧
-    (Main[46] = 0 ∨ Main[46] = 1) ∧
-    (Main[47] = 0 ∨ Main[40] + Main[41] * 2 * 1 = 2) ∧
-    (Main[47] = 0 ∨ Main[47] = 1) ∧
-    (Main[48] = 0 ∨ Main[40] + Main[41] * 2 * 1 = 3) ∧
-    (Main[48] = 0 ∨ Main[48] = 1) ∧
-    (Main[45] + Main[46] + Main[47] + Main[48] = 1) ∧
-    (Main[42] = (Main[36] + 1) * (Main[37] * 3 + 1)) ∧
-    (Main[43] = Main[42] * (Main[38] * 15 + 1)) ∧
-    (Main[44] = Main[43] * (Main[39] * 255 + 1)) ∧
-    (Main[49].val < 2 ^ ((16 : Fin BB) - (Main[36] + Main[37] * 2 + Main[38] * 4 + Main[39] * 8)).val) ∧
-    (Main[53].val < 2 ^ (Main[36] + Main[37] * 2 + Main[38] * 4 + Main[39] * 8).val) ∧
-    (Main[15] * Main[44] = Main[53] * 65536 + Main[49] * Main[44]) ∧
-    (Main[50].val < 2 ^ ((16 : Fin BB) - (Main[36] + Main[37] * 2 + Main[38] * 4 + Main[39] * 8)).val) ∧
-    (Main[54].val < 2 ^ (Main[36] + Main[37] * 2 + Main[38] * 4 + Main[39] * 8).val) ∧
-    (Main[16] * Main[44] = Main[54] * 65536 + Main[50] * Main[44]) ∧
-    (Main[51].val < 2 ^ ((16 : Fin BB) - (Main[36] + Main[37] * 2 + Main[38] * 4 + Main[39] * 8)).val) ∧
-    (Main[55].val < 2 ^ (Main[36] + Main[37] * 2 + Main[38] * 4 + Main[39] * 8).val) ∧
-    (Main[17] * Main[44] = Main[55] * 65536 + Main[51] * Main[44]) ∧
-    (Main[52].val < 2 ^ ((16 : Fin BB) - (Main[36] + Main[37] * 2 + Main[38] * 4 + Main[39] * 8)).val) ∧
-    (Main[56].val < 2 ^ (Main[36] + Main[37] * 2 + Main[38] * 4 + Main[39] * 8).val) ∧
-    (Main[18] * Main[44] = Main[56] * 65536 + Main[52] * Main[44]) ∧
-    (Main[57] = Main[49] * Main[44]) ∧
-    (Main[58] = Main[50] * Main[44] + Main[53]) ∧
-    (Main[59] = Main[51] * Main[44] + Main[54]) ∧
-    (Main[60] = Main[52] * Main[44] + Main[55]) ∧
-    (Main[45] = 0 ∨ Main[32] = Main[57]) ∧
-    (Main[45] = 0 ∨ Main[33] = Main[58]) ∧
-    (Main[45] = 0 ∨ Main[34] = Main[59]) ∧
-    (Main[45] = 0 ∨ Main[35] = Main[60]) ∧
-    (Main[46] = 0 ∨ Main[32] = 0) ∧
-    (Main[46] = 0 ∨ Main[33] = Main[57]) ∧
-    (Main[46] = 0 ∨ Main[34] = Main[58]) ∧
-    (Main[46] = 0 ∨ Main[35] = Main[59]) ∧
-    (Main[47] = 0 ∨ Main[32] = 0) ∧
-    (Main[47] = 0 ∨ Main[33] = 0) ∧
-    (Main[47] = 0 ∨ Main[34] = Main[57]) ∧
-    (Main[47] = 0 ∨ Main[35] = Main[58]) ∧
-    (Main[48] = 0 ∨ Main[32] = 0) ∧
-    (Main[48] = 0 ∨ Main[33] = 0) ∧
-    (Main[48] = 0 ∨ Main[34] = 0) ∧
-    (Main[48] = 0 ∨ Main[35] = Main[57]) ∧
-    (Main[63] = 0) ∧
-    (Main[64] = 19)
-   := by
-  obtain ⟨ m62, m31 ⟩ := h
-  simp_all [allHold_constraints_iff, constraints, sub_eq_zero]
-  constructor <;> intro cstrs
-  . obtain ⟨ msb, cpu, alu,
-             b_m62, b_m63,
-             b_m36, b_m37, b_m38, b_m39, b_m40, b_m41,
-             diff_m25,
-             eq_m45, b_m45, eq_m46, b_m46, eq_m47, b_m47, eq_m48, b_m48,
-             one_of_45_46_47_48,
-             eq_m42, eq_m43, eq_m44,
-             lt_m49, lt_m53, h_15_44,
-             lt_m50, lt_m54, h_16_44,
-             lt_m51, lt_m55, h_17_44,
-             lt_m52, lt_m56, h_18_44,
-             eq_m57, eq_m58, eq_m59, eq_m60,
-             sll_00, sll_01, sll_02, sll_03, sll_04, sll_05, sll_06, sll_07, sll_08, sll_09, sll_10, sll_11, sll_12, sll_13, sll_14, sll_15,
-             sllw_00, sllw_01, sllw_02, sllw_03, sllw_04, sllw_05,
-             eq_m64 ⟩ := cstrs
-    have : Main[63] = 0 := by clear *- b_m62 b_m63; aesop
-    simp_all
-  . obtain ⟨ msb, cpu, alu,
-             b_m36, b_m37, b_m38, b_m39, b_m40, b_m41,
-             diff_m25,
-             eq_m45, b_m45, eq_m46, b_m46, eq_m47, b_m47, eq_m48, b_m48,
-             one_of_45_46_47_48,
-             eq_m42, eq_m43, eq_m44,
-             lt_m49, lt_m53, h_15_44,
-             lt_m50, lt_m54, h_16_44,
-             lt_m51, lt_m55, h_17_44,
-             lt_m52, lt_m56, h_18_44,
-             eq_m57, eq_m58, eq_m59, eq_m60,
-             sll_00, sll_01, sll_02, sll_03, sll_04, sll_05, sll_06, sll_07, sll_08, sll_09, sll_10, sll_11, sll_12, sll_13, sll_14, sll_15,
-             eq_m63, eq_m64 ⟩ := cstrs
-    simp_all
-
 set_option maxHeartbeats 100000000 in
 lemma spec.slli (h : is_slli Main) :
   List.Forall SP1Constraint.toProp (constraints Main) →
     Main[25] < 64 ∧ Main[26] = 0 ∧ Main[27] = 0 ∧ Main[28] = 0 ∧
     Word.toBitVec64 #v[Main[32], Main[33], Main[34], Main[35]] = execute_RTYPE_pure_w #v[Main[15], Main[16], Main[17], Main[18]] #v[Main[25], Main[26], Main[27], Main[28]] .SLL
-  := by
-    intro cstrs; rw [allHold_constraints_iff_slli h] at cstrs
-
-    set b0 := Main[15]
-    set b1 := Main[16]
-    set b2 := Main[17]
-    set b3 := Main[18]
-    set c0 := Main[25]
-    set c1 := Main[26]
-    set c2 := Main[27]
-    set c3 := Main[28]
-    set a0 := Main[32]
-    set a1 := Main[33]
-    set a2 := Main[34]
-    set a3 := Main[35]
-    set cb0 := Main[36]
-    set cb1 := Main[37]
-    set cb2 := Main[38]
-    set cb3 := Main[39]
-    set cb4 := Main[40]
-    set cb5 := Main[41]
-    set v01 := Main[42]
-    set v012 := Main[43]
-    set v0123 := Main[44]
-    set su160 := Main[45]
-    set su161 := Main[46]
-    set su162 := Main[47]
-    set su163 := Main[48]
-    set ll0 := Main[49]
-    set ll1 := Main[50]
-    set ll2 := Main[51]
-    set ll3 := Main[52]
-    set hl0 := Main[53]
-    set hl1 := Main[54]
-    set hl2 := Main[55]
-    set hl3 := Main[56]
-    set lr0 := Main[57]
-    set lr1 := Main[58]
-    set lr2 := Main[59]
-    set lr3 := Main[60]
-    set msb := Main[61]
-
-    obtain ⟨ eq_m62, eq_m31 ⟩ := h
-    obtain ⟨ msb_cstrs, cpu_cstrs, alu_cstrs,
-             b_cb0, b_cb1, b_cb2, b_cb3, b_cb4, b_cb5,
-             diff,
-             eq_su160, b_su160, eq_su161, b_su161, eq_su162, b_su162, eq_su163, b_su163,
-             one_of_su16,
-             eq_v01, eq_v012, eq_v0123,
-             lt_ll0, lt_hl0, h_b0_dec,
-             lt_ll1, lt_hl1, h_b1_dec,
-             lt_ll2, lt_hl2, h_b2_dec,
-             lt_ll3, lt_hl3, h_b3_dec,
-             eq_lr0, eq_lr1, eq_lr2, eq_lr3,
-             sll_00, sll_01, sll_02, sll_03, sll_04, sll_05, sll_06, sll_07, sll_08, sll_09, sll_10, sll_11, sll_12, sll_13, sll_14, sll_15,
-             eq_m63, eq_m64 ⟩ := cstrs
-    clear msb_cstrs cpu_cstrs
-    rw [ALUTypeReader.allHold_constraints_iff_is_real (by rfl)] at alu_cstrs
-    simp [Opcode.ofNat, Nat.ble, Nat.beq] at alu_cstrs
-    obtain ⟨ ⟨ h0, hc0, hc1, hc2, hc3 ⟩, h1, h2, h3, h4, h5, h6, h7, h8, h9, h10, h11, h12, h13, h14, is_U64_b, h15, eq_c0, eq_c1, eq_c2, eq_c3 ⟩ := alu_cstrs
-    clear h0 h1 h2 h3 h4 h5 h6 h7 h8 h9 h10 h11 h12 h13 h14 h15
-    rw [← eq_c0] at hc0 eq_c0; simp_all
-
-    have ⟨ b0_16, b1_16, b2_16, b3_16 ⟩ := Word.lt_cases_of_isU64 is_U64_b
-    simp_all
-
-    have is_U64_b : Word.isU64 #v[ b0, b1, b2, b3 ] := by apply Word.isU64_of_cases <;> assumption
-    have is_U64_c : Word.isU64 #v[ c0, 0, 0, 0 ] := by apply Word.isU64_of_cases <;> simp; omega
-
-    have ⟨ b0_16, b1_16, b2_16, b3_16 ⟩ := Word.lt_cases_of_isU64 is_U64_b
-    simp_all
-
-
-
-
-    -- rw [← BitVec.toNat_inj, BitVec.toNat_shiftLeft, Nat.shiftLeft_eq]
-
-    -- have : ((Word.toBitVec64 #v[c0, 0, 0, 0]).toNat % 64) = c0.val % 64 := by
-    --   rw [Word.toBitVec64_toNat is_U64_c]; simp [Word.toNat]
-    -- rw [this]; clear this
-    -- have : c0.val % 64 = cb0.val + cb1.val * 2 + cb2.val * 4 + cb3.val * 8 + cb4.val * 16 + cb5.val * 32 := by
-    --   rw [is_mod_64 (m := cb0 + cb1 * 2 + cb2 * 4 + cb3 * 8 + cb4 * 16 + cb5 * 32)]
-    --   . clear *- b_cb0 b_cb1 b_cb2 b_cb3 b_cb4 b_cb5
-    --     omega
-    --   . clear *- b_cb0 b_cb1 b_cb2 b_cb3 b_cb4 b_cb5
-    --     omega
-    --   . omega
-    --   . exact diff
-
-    -- rw [this]; clear this
-    -- rw [Word.toBitVec64_toNat (w := #v[b0, b1, b2, b3]) (by apply Word.isU64_of_cases <;> simp <;> assumption)]
-    -- simp [Word.toNat]
-
-    sorry
-
-    -- -- 64-way case split
-    -- rcases b_cb0 <;> rcases b_cb1 <;> rcases b_cb2 <;>
-    -- rcases b_cb3 <;> rcases b_cb4 <;> rcases b_cb5 <;>
-    -- simp_all <;>
-    -- (try apply cancel_mul_65536 (by simp) at h_b0_dec) <;>
-    -- (try apply cancel_mul_65536 (by simp) at h_b1_dec) <;>
-    -- (try apply cancel_mul_65536 (by simp) at h_b2_dec) <;>
-    -- (try apply cancel_mul_65536 (by simp) at h_b3_dec) <;>
-    -- simp_all
-
-    -- all_goals {
-    --   rw [Word.toBitVec64_toNat]
-    --   . simp [Word.toNat]
-    --     try simp [Fin.val_add, Fin.val_mul] at b0_16 b1_16 b2_16 b3_16 ⊢
-    --     repeat rw [Nat.mod_eq_of_lt (b := 2013265921) (by omega)]
-    --     omega
-    --   . apply Word.isU64_of_cases <;> simp [Fin.val_add, Fin.val_mul] <;>
-    --     (repeat rw [Nat.mod_eq_of_lt (b := 2013265921) (by omega)]) <;>
-    --     omega
-    -- }
-
-end slli
-
-section sllw
-
-@[simp] def is_sllw (Main : Vector (Fin BB) 65) := Main[63] = 1 ∧ Main[31] = 0
-
-set_option maxHeartbeats 1000000 in
-lemma allHold_constraints_iff_sllw (h : is_sllw Main) :
-  List.Forall SP1Constraint.toProp (constraints Main) ↔
-    List.Forall SP1Constraint.toProp (U16MSBOperation.constraints Main[33] { msb := Main[61] } 1) ∧
-    List.Forall SP1Constraint.toProp (CPUState.constraints { clk_high := Main[0], clk_16_24 := Main[1], clk_0_16 := Main[2], pc := #v[Main[3], Main[4], Main[5]] } #v[Main[3] + 4, Main[4], Main[5]] 8 1) ∧
-    List.Forall SP1Constraint.toProp (ALUTypeReader.constraints Main[0] (Main[2] + Main[1] * 65536) #v[Main[3], Main[4], Main[5]] 41 #v[Main[64], 1, 0] #v[Main[32], Main[33], Main[34], Main[35]] { op_a := Main[6], op_a_memory := { prev_value := #v[Main[7], Main[8], Main[9], Main[10]], access_timestamp := { prev_low := Main[11], diff_low_limb := Main[12] } }, op_a_0 := Main[13], op_b := Main[14], op_b_memory := { prev_value := #v[Main[15], Main[16], Main[17], Main[18]], access_timestamp := { prev_low := Main[19], diff_low_limb := Main[20] } }, op_c := #v[Main[21], Main[22], Main[23], Main[24]], op_c_memory := { prev_value := #v[Main[25], Main[26], Main[27], Main[28]], access_timestamp := { prev_low := Main[29], diff_low_limb := Main[30] } }, imm_c := 0 } 1) ∧
-    (Main[36] = 0 ∨ Main[36] = 1) ∧
-    (Main[37] = 0 ∨ Main[37] = 1) ∧
-    (Main[38] = 0 ∨ Main[38] = 1) ∧
-    (Main[39] = 0 ∨ Main[39] = 1) ∧
-    (Main[40] = 0 ∨ Main[40] = 1) ∧
-    (Main[41] = 0 ∨ Main[41] = 1) ∧
-    (((Main[25] - (Main[36] + Main[37] * 2 + Main[38] * 4 + Main[39] * 8 + Main[40] * 16 + Main[41] * 32)) * 1981808641).val < 1024) ∧
-    (Main[45] = 0 ∨ Main[40] = 0) ∧
-    (Main[45] = 0 ∨ Main[45] = 1) ∧
-    (Main[46] = 0 ∨ Main[40] = 1) ∧
-    (Main[46] = 0 ∨ Main[46] = 1) ∧
-    (Main[47] = 0 ∨ Main[40] = 2) ∧
-    (Main[47] = 0 ∨ Main[47] = 1) ∧
-    (Main[48] = 0 ∨ Main[40] = 3) ∧
-    (Main[48] = 0 ∨ Main[48] = 1) ∧
-    (Main[45] + Main[46] + Main[47] + Main[48] = 1) ∧
-    (Main[42] = (Main[36] + 1) * (Main[37] * 3 + 1)) ∧
-    (Main[43] = Main[42] * (Main[38] * 15 + 1)) ∧
-    (Main[44] = Main[43] * (Main[39] * 255 + 1)) ∧
-    (Main[49].val < 2 ^ ((16 : Fin BB) - (Main[36] + Main[37] * 2 + Main[38] * 4 + Main[39] * 8)).val) ∧
-    (Main[53].val < 2 ^ (Main[36] + Main[37] * 2 + Main[38] * 4 + Main[39] * 8).val) ∧
-    (Main[15] * Main[44] = Main[53] * 65536 + Main[49] * Main[44]) ∧
-    (Main[50].val < 2 ^ ((16 : Fin BB) - (Main[36] + Main[37] * 2 + Main[38] * 4 + Main[39] * 8)).val) ∧
-    (Main[54].val < 2 ^ (Main[36] + Main[37] * 2 + Main[38] * 4 + Main[39] * 8).val) ∧
-    (Main[16] * Main[44] = Main[54] * 65536 + Main[50] * Main[44]) ∧
-    (Main[51].val < 2 ^ ((16 : Fin BB) - (Main[36] + Main[37] * 2 + Main[38] * 4 + Main[39] * 8)).val) ∧
-    (Main[55].val < 2 ^ (Main[36] + Main[37] * 2 + Main[38] * 4 + Main[39] * 8).val) ∧
-    (Main[17] * Main[44] = Main[55] * 65536 + Main[51] * Main[44]) ∧
-    (Main[52].val < 2 ^ ((16 : Fin BB) - (Main[36] + Main[37] * 2 + Main[38] * 4 + Main[39] * 8)).val) ∧
-    (Main[56].val < 2 ^ (Main[36] + Main[37] * 2 + Main[38] * 4 + Main[39] * 8).val) ∧
-    (Main[18] * Main[44] = Main[56] * 65536 + Main[52] * Main[44]) ∧
-    (Main[57] = Main[49] * Main[44]) ∧
-    (Main[58] = Main[50] * Main[44] + Main[53]) ∧
-    (Main[59] = Main[51] * Main[44] + Main[54]) ∧
-    (Main[60] = Main[52] * Main[44] + Main[55]) ∧
-    (Main[45] = 0 ∨ Main[32] = Main[57]) ∧
-    (Main[45] = 0 ∨ Main[33] = Main[58]) ∧
-    (Main[46] = 0 ∨ Main[32] = 0) ∧
-    (Main[46] = 0 ∨ Main[33] = Main[57]) ∧
-    (Main[61] * 65535 = Main[34]) ∧
-    (Main[61] * 65535 = Main[35]) ∧
-    (Main[62] = 0) ∧
-    (Main[64] = 59)
-   := by
-  obtain ⟨ m63, m31 ⟩ := h
-  simp_all [allHold_constraints_iff, constraints, sub_eq_zero]
-  intro msb
-  constructor <;> intro cstrs
-  . obtain ⟨ cpu, alu,
-             b_m62, b_m63,
-             b_m36, b_m37, b_m38, b_m39, b_m40, b_m41,
-             diff_m25,
-             eq_m45, b_m45, eq_m46, b_m46, eq_m47, b_m47, eq_m48, b_m48,
-             one_of_45_46_47_48,
-             eq_m42, eq_m43, eq_m44,
-             lt_m49, lt_m53, h_15_44,
-             lt_m50, lt_m54, h_16_44,
-             lt_m51, lt_m55, h_17_44,
-             lt_m52, lt_m56, h_18_44,
-             eq_m57, eq_m58, eq_m59, eq_m60,
-             sll_00, sll_01, sll_02, sll_03, sll_04, sll_05, sll_06, sll_07, sll_08, sll_09, sll_10, sll_11, sll_12, sll_13, sll_14, sll_15,
-             sllw_00, sllw_01, sllw_02, sllw_03, sllw_04, sllw_05,
-             eq_m64 ⟩ := cstrs
-    have : Main[62] = 0 := by clear *- b_m62 b_m63; aesop
-    simp_all
-  . obtain ⟨ cpu, alu,
-             b_m36, b_m37, b_m38, b_m39, b_m40, b_m41,
-             diff_m25,
-             eq_m45, b_m45, eq_m46, b_m46, eq_m47, b_m47, eq_m48, b_m48,
-             one_of_45_46_47_48,
-             eq_m42, eq_m43, eq_m44,
-             lt_m49, lt_m53, h_15_44,
-             lt_m50, lt_m54, h_16_44,
-             lt_m51, lt_m55, h_17_44,
-             lt_m52, lt_m56, h_18_44,
-             eq_m57, eq_m58, eq_m59, eq_m60,
-             sllw_00, sllw_01, sllw_02, sllw_03, sllw_04, sllw_05,
-             eq_m62, eq_m64 ⟩ := cstrs
-    simp_all
-
-set_option maxHeartbeats 100000000 in
-lemma spec.sllw (h : is_sllw Main) :
-  List.Forall SP1Constraint.toProp (constraints Main) →
-    Word.toBitVec64 #v[Main[32], Main[33], Main[34], Main[35]] = execute_RTYPEW_pure_w #v[Main[15], Main[16], Main[17], Main[18]] #v[Main[25], Main[26], Main[27], Main[28]] .SLLW
   := by sorry
-    -- intro cstrs; rw [allHold_constraints_iff_sllw h] at cstrs
+    -- intro cstrs; rw [allHold_constraints_iff] at cstrs
+    -- obtain ⟨ eq_sll, eq_imm ⟩ := h
 
     -- set b0 := Main[15]
     -- set b1 := Main[16]
@@ -924,6 +538,7 @@ lemma spec.sllw (h : is_sllw Main) :
     -- set c1 := Main[26]
     -- set c2 := Main[27]
     -- set c3 := Main[28]
+    -- set imm := Main[31]
     -- set a0 := Main[32]
     -- set a1 := Main[33]
     -- set a2 := Main[34]
@@ -954,25 +569,158 @@ lemma spec.sllw (h : is_sllw Main) :
     -- set lr2 := Main[59]
     -- set lr3 := Main[60]
     -- set msb := Main[61]
+    -- set sll := Main[62]
+    -- set sllw := Main[63]
 
-    -- obtain ⟨ eq_m63, eq_m31 ⟩ := h
-    -- obtain ⟨ msb_cstrs, cpu_cstrs, alu_cstrs,
-    --          b_cb0, b_cb1, b_cb2, b_cb3, b_cb4, b_cb5,
-    --          diff,
-    --          eq_su160, b_su160, eq_su161, b_su161, eq_su162, b_su162, eq_su163, b_su163,
-    --          one_of_su16,
+    -- obtain ⟨ msb_a1, cpu, alu, one_of_ops,
+    --          b_sll, b_sllw,
+    --          b_cb0, b_cb1, b_cb2, b_cb3, b_cb4, b_cb5, diff,
+    --          h_su160, b_su160, h_su161, b_su161, h_su162, b_su162, h_su163, b_su163, one_of_su16s,
     --          eq_v01, eq_v012, eq_v0123,
-    --          lt_ll0, lt_hl0, h_b0_dec,
-    --          lt_ll1, lt_hl1, h_b1_dec,
-    --          lt_ll2, lt_hl2, h_b2_dec,
-    --          lt_ll3, lt_hl3, h_b3_dec,
+    --          lt_ll0, lt_lh0, h_b0_dec, lt_ll1, lt_lh1, h_b1_dec,
+    --          lt_ll2, lt_lh2, h_b2_dec, lt_ll3, lt_lh3, h_b3_dec,
     --          eq_lr0, eq_lr1, eq_lr2, eq_lr3,
-    --          sllw_00, sllw_01, sllw_02, sllw_03, sllw_04, sllw_05,
-    --          eq_m62, eq_m64 ⟩ := cstrs
-    -- clear cpu_cstrs
-    -- rw [ALUTypeReader.allHold_constraints_iff_is_real (by rfl)] at alu_cstrs
-    -- simp [Opcode.ofNat, Nat.ble, Nat.beq] at alu_cstrs
-    -- obtain ⟨ h0, h1, h2, h3, h4, h5, h6, h7, h8, h9, h10, h11, h12, h13, h14, is_U64_b, ⟨ h15, h16, is_U64_c ⟩, h17 ⟩ := alu_cstrs
+    --          nw_00, nw_01, nw_02, nw_03, nw_04, nw_05, nw_06, nw_07, nw_08, nw_09, nw_10, nw_11, nw_12, nw_13, nw_14, nw_15,
+    --          w_00, w_01, w_02, w_03, w_04, w_05,
+    --          eq_m64 ⟩ := cstrs
+
+    -- have eq_m63 : sllw = 0 := by
+    --   clear *- b_sll b_sllw one_of_ops eq_sll
+    --   simp_all; aesop
+
+    -- simp_all
+
+    -- clear msb_a1 cpu
+    -- rw [ALUTypeReader.allHold_constraints_iff_is_real (by rfl)] at alu
+    -- simp [Opcode.ofNat, Nat.ble, Nat.beq] at alu
+    -- obtain ⟨ ⟨ h0, hc0, hc1, hc2, hc3 ⟩, h1, h2, h3, h4, h5, h6, h7, h8, h9, h10, h11, h12, h13, h14, is_U64_b, h15, eq_c0, eq_c1, eq_c2, eq_c3 ⟩ := alu
+    -- clear h0 h1 h2 h3 h4 h5 h6 h7 h8 h9 h10 h11 h12 h13 h14 h15
+    -- rw [← eq_c0] at hc0 eq_c0; simp_all
+
+    -- have ⟨ b0_16, b1_16, b2_16, b3_16 ⟩ := Word.lt_cases_of_isU64 is_U64_b
+    -- simp_all
+
+    -- have is_U64_b : Word.isU64 #v[ b0, b1, b2, b3 ] := by apply Word.isU64_of_cases <;> assumption
+    -- have is_U64_c : Word.isU64 #v[ c0, 0, 0, 0 ] := by apply Word.isU64_of_cases <;> simp; omega
+
+    -- have ⟨ b0_16, b1_16, b2_16, b3_16 ⟩ := Word.lt_cases_of_isU64 is_U64_b
+    -- simp_all
+
+    -- rw [← BitVec.toNat_inj, BitVec.toNat_shiftLeft, Nat.shiftLeft_eq]
+
+    -- have : ((Word.toBitVec64 #v[c0, 0, 0, 0]).toNat % 64) = c0.val % 64 := by
+    --   rw [Word.toBitVec64_toNat is_U64_c]; simp [Word.toNat]
+    -- rw [this]; clear this
+    -- have : c0.val % 64 = cb0.val + cb1.val * 2 + cb2.val * 4 + cb3.val * 8 + cb4.val * 16 + cb5.val * 32 := by
+    --   rw [is_mod_64 (m := cb0 + cb1 * 2 + cb2 * 4 + cb3 * 8 + cb4 * 16 + cb5 * 32)]
+    --   . clear *- b_cb0 b_cb1 b_cb2 b_cb3 b_cb4 b_cb5
+    --     omega
+    --   . clear *- b_cb0 b_cb1 b_cb2 b_cb3 b_cb4 b_cb5
+    --     omega
+    --   . omega
+    --   . exact diff
+
+    -- rw [this]; clear this
+    -- rw [Word.toBitVec64_toNat (w := #v[b0, b1, b2, b3]) (by apply Word.isU64_of_cases <;> simp <;> assumption)]
+    -- simp [Word.toNat]
+
+    -- -- 64-way case split
+    -- rcases b_cb0 <;> rcases b_cb1 <;> rcases b_cb2 <;>
+    -- rcases b_cb3 <;> rcases b_cb4 <;> rcases b_cb5 <;>
+    -- simp_all <;>
+    -- (try apply cancel_mul_65536 (by simp) at h_b0_dec) <;>
+    -- (try apply cancel_mul_65536 (by simp) at h_b1_dec) <;>
+    -- (try apply cancel_mul_65536 (by simp) at h_b2_dec) <;>
+    -- (try apply cancel_mul_65536 (by simp) at h_b3_dec) <;>
+    -- simp_all
+
+    -- all_goals {
+    --   rw [Word.toBitVec64_toNat]
+    --   . simp [Word.toNat]
+    --     try simp [Fin.val_add, Fin.val_mul] at b0_16 b1_16 b2_16 b3_16 ⊢
+    --     repeat rw [Nat.mod_eq_of_lt (b := 2013265921) (by omega)]
+    --     omega
+    --   . apply Word.isU64_of_cases <;> simp [Fin.val_add, Fin.val_mul] <;>
+    --     (repeat rw [Nat.mod_eq_of_lt (b := 2013265921) (by omega)]) <;>
+    --     omega
+    -- }
+
+end slli
+
+section sllw
+
+set_option maxHeartbeats 100000000 in
+lemma spec.sllw (h : is_sllw Main) :
+  List.Forall SP1Constraint.toProp (constraints Main) →
+    Word.toBitVec64 #v[Main[32], Main[33], Main[34], Main[35]] = execute_RTYPEW_pure_w #v[Main[15], Main[16], Main[17], Main[18]] #v[Main[25], Main[26], Main[27], Main[28]] .SLLW
+  := by sorry
+    -- intro cstrs; rw [allHold_constraints_iff] at cstrs
+    -- obtain ⟨ eq_sllw, eq_imm ⟩ := h
+
+    -- set b0 := Main[15]
+    -- set b1 := Main[16]
+    -- set b2 := Main[17]
+    -- set b3 := Main[18]
+    -- set c0 := Main[25]
+    -- set c1 := Main[26]
+    -- set c2 := Main[27]
+    -- set c3 := Main[28]
+    -- set imm := Main[31]
+    -- set a0 := Main[32]
+    -- set a1 := Main[33]
+    -- set a2 := Main[34]
+    -- set a3 := Main[35]
+    -- set cb0 := Main[36]
+    -- set cb1 := Main[37]
+    -- set cb2 := Main[38]
+    -- set cb3 := Main[39]
+    -- set cb4 := Main[40]
+    -- set cb5 := Main[41]
+    -- set v01 := Main[42]
+    -- set v012 := Main[43]
+    -- set v0123 := Main[44]
+    -- set su160 := Main[45]
+    -- set su161 := Main[46]
+    -- set su162 := Main[47]
+    -- set su163 := Main[48]
+    -- set ll0 := Main[49]
+    -- set ll1 := Main[50]
+    -- set ll2 := Main[51]
+    -- set ll3 := Main[52]
+    -- set hl0 := Main[53]
+    -- set hl1 := Main[54]
+    -- set hl2 := Main[55]
+    -- set hl3 := Main[56]
+    -- set lr0 := Main[57]
+    -- set lr1 := Main[58]
+    -- set lr2 := Main[59]
+    -- set lr3 := Main[60]
+    -- set msb := Main[61]
+    -- set sll := Main[62]
+    -- set sllw := Main[63]
+
+    -- obtain ⟨ msb_a1, cpu, alu, one_of_ops,
+    --          b_sll, b_sllw,
+    --          b_cb0, b_cb1, b_cb2, b_cb3, b_cb4, b_cb5, diff,
+    --          h_su160, b_su160, h_su161, b_su161, h_su162, b_su162, h_su163, b_su163, one_of_su16s,
+    --          eq_v01, eq_v012, eq_v0123,
+    --          lt_ll0, lt_lh0, h_b0_dec, lt_ll1, lt_lh1, h_b1_dec,
+    --          lt_ll2, lt_lh2, h_b2_dec, lt_ll3, lt_lh3, h_b3_dec,
+    --          eq_lr0, eq_lr1, eq_lr2, eq_lr3,
+    --          nw_00, nw_01, nw_02, nw_03, nw_04, nw_05, nw_06, nw_07, nw_08, nw_09, nw_10, nw_11, nw_12, nw_13, nw_14, nw_15,
+    --          w_00, w_01, w_02, w_03, w_04, w_05,
+    --          eq_m64 ⟩ := cstrs
+
+    -- have eq_m63 : sll = 0 := by
+    --   clear *- b_sll b_sllw one_of_ops eq_sllw
+    --   simp_all; aesop
+
+    -- simp_all
+
+    -- clear cpu
+    -- rw [ALUTypeReader.allHold_constraints_iff_is_real (by rfl)] at alu
+    -- simp [Opcode.ofNat, Nat.ble, Nat.beq] at alu
+    -- obtain ⟨ h0, h1, h2, h3, h4, h5, h6, h7, h8, h9, h10, h11, h12, h13, h14, is_U64_b, ⟨ h15, h16, is_U64_c ⟩, h17 ⟩ := alu
     -- clear h0 h1 h2 h3 h4 h5 h6 h7 h8 h9 h10 h11 h12 h13 h14 h15 h16 h17
     -- simp_all
 
@@ -1017,8 +765,9 @@ lemma spec.sllw (h : is_sllw Main) :
     -- have ⟨ _, _ ⟩ := HalfWord.lt_cases_of_isU32 h_isU32_a
 
     -- have h_a3 : a3 = if (HalfWord.toBitVec32 #v[a0, a1]).msb = true then 65535 else 0 := by
-    --   rw [← sllw_05, ← sllw_04]
-    --   have h_msb := U16MSBOperation.spec a1 { msb := msb } 1 (by assumption) msb_cstrs (by simp)
+    --   simp_all
+    --   rw [← w_04] at *
+    --   have h_msb := U16MSBOperation.spec a1 { msb := msb } 1 (by assumption) msb_a1 (by simp)
     --   simp at h_msb; rw [h_msb]
     --   trans (if HalfWord.isNegative #v[a0, a1] then 65535 else 0)
     --   . unfold HalfWord.isNegative; split_ifs <;> simp_all; omega
@@ -1050,103 +799,14 @@ end sllw
 
 section slliw
 
-@[simp] def is_slliw (Main : Vector (Fin BB) 65) := Main[63] = 1 ∧ Main[31] = 1
-
-set_option maxHeartbeats 1000000 in
-lemma allHold_constraints_iff_slliw (h : is_slliw Main) :
-  List.Forall SP1Constraint.toProp (constraints Main) ↔
-    List.Forall SP1Constraint.toProp (U16MSBOperation.constraints Main[33] { msb := Main[61] } 1) ∧
-    List.Forall SP1Constraint.toProp (CPUState.constraints { clk_high := Main[0], clk_16_24 := Main[1], clk_0_16 := Main[2], pc := #v[Main[3], Main[4], Main[5]] } #v[Main[3] + 4, Main[4], Main[5]] 8 1) ∧
-    List.Forall SP1Constraint.toProp (ALUTypeReader.constraints Main[0] (Main[2] + Main[1] * 65536) #v[Main[3], Main[4], Main[5]] 41 #v[Main[64], 1, 0] #v[Main[32], Main[33], Main[34], Main[35]] { op_a := Main[6], op_a_memory := { prev_value := #v[Main[7], Main[8], Main[9], Main[10]], access_timestamp := { prev_low := Main[11], diff_low_limb := Main[12] } }, op_a_0 := Main[13], op_b := Main[14], op_b_memory := { prev_value := #v[Main[15], Main[16], Main[17], Main[18]], access_timestamp := { prev_low := Main[19], diff_low_limb := Main[20] } }, op_c := #v[Main[21], Main[22], Main[23], Main[24]], op_c_memory := { prev_value := #v[Main[25], Main[26], Main[27], Main[28]], access_timestamp := { prev_low := Main[29], diff_low_limb := Main[30] } }, imm_c := 1 } 1) ∧
-    (Main[36] = 0 ∨ Main[36] = 1) ∧
-    (Main[37] = 0 ∨ Main[37] = 1) ∧
-    (Main[38] = 0 ∨ Main[38] = 1) ∧
-    (Main[39] = 0 ∨ Main[39] = 1) ∧
-    (Main[40] = 0 ∨ Main[40] = 1) ∧
-    (Main[41] = 0 ∨ Main[41] = 1) ∧
-    (((Main[25] - (Main[36] + Main[37] * 2 + Main[38] * 4 + Main[39] * 8 + Main[40] * 16 + Main[41] * 32)) * 1981808641).val < 1024) ∧
-    (Main[45] = 0 ∨ Main[40] = 0) ∧
-    (Main[45] = 0 ∨ Main[45] = 1) ∧
-    (Main[46] = 0 ∨ Main[40] = 1) ∧
-    (Main[46] = 0 ∨ Main[46] = 1) ∧
-    (Main[47] = 0 ∨ Main[40] = 2) ∧
-    (Main[47] = 0 ∨ Main[47] = 1) ∧
-    (Main[48] = 0 ∨ Main[40] = 3) ∧
-    (Main[48] = 0 ∨ Main[48] = 1) ∧
-    (Main[45] + Main[46] + Main[47] + Main[48] = 1) ∧
-    (Main[42] = (Main[36] + 1) * (Main[37] * 3 + 1)) ∧
-    (Main[43] = Main[42] * (Main[38] * 15 + 1)) ∧
-    (Main[44] = Main[43] * (Main[39] * 255 + 1)) ∧
-    (Main[49].val < 2 ^ ((16 : Fin BB) - (Main[36] + Main[37] * 2 + Main[38] * 4 + Main[39] * 8)).val) ∧
-    (Main[53].val < 2 ^ (Main[36] + Main[37] * 2 + Main[38] * 4 + Main[39] * 8).val) ∧
-    (Main[15] * Main[44] = Main[53] * 65536 + Main[49] * Main[44]) ∧
-    (Main[50].val < 2 ^ ((16 : Fin BB) - (Main[36] + Main[37] * 2 + Main[38] * 4 + Main[39] * 8)).val) ∧
-    (Main[54].val < 2 ^ (Main[36] + Main[37] * 2 + Main[38] * 4 + Main[39] * 8).val) ∧
-    (Main[16] * Main[44] = Main[54] * 65536 + Main[50] * Main[44]) ∧
-    (Main[51].val < 2 ^ ((16 : Fin BB) - (Main[36] + Main[37] * 2 + Main[38] * 4 + Main[39] * 8)).val) ∧
-    (Main[55].val < 2 ^ (Main[36] + Main[37] * 2 + Main[38] * 4 + Main[39] * 8).val) ∧
-    (Main[17] * Main[44] = Main[55] * 65536 + Main[51] * Main[44]) ∧
-    (Main[52].val < 2 ^ ((16 : Fin BB) - (Main[36] + Main[37] * 2 + Main[38] * 4 + Main[39] * 8)).val) ∧
-    (Main[56].val < 2 ^ (Main[36] + Main[37] * 2 + Main[38] * 4 + Main[39] * 8).val) ∧
-    (Main[18] * Main[44] = Main[56] * 65536 + Main[52] * Main[44]) ∧
-    (Main[57] = Main[49] * Main[44]) ∧
-    (Main[58] = Main[50] * Main[44] + Main[53]) ∧
-    (Main[59] = Main[51] * Main[44] + Main[54]) ∧
-    (Main[60] = Main[52] * Main[44] + Main[55]) ∧
-    (Main[45] = 0 ∨ Main[32] = Main[57]) ∧
-    (Main[45] = 0 ∨ Main[33] = Main[58]) ∧
-    (Main[46] = 0 ∨ Main[32] = 0) ∧
-    (Main[46] = 0 ∨ Main[33] = Main[57]) ∧
-    (Main[61] * 65535 = Main[34]) ∧
-    (Main[61] * 65535 = Main[35]) ∧
-    (Main[62] = 0) ∧
-    (Main[64] = 27)
-   := by
-  obtain ⟨ m63, m31 ⟩ := h
-  simp_all [allHold_constraints_iff, constraints, sub_eq_zero]
-  intro msb
-  constructor <;> intro cstrs
-  . obtain ⟨ cpu, alu,
-             b_m62, b_m63,
-             b_m36, b_m37, b_m38, b_m39, b_m40, b_m41,
-             diff_m25,
-             eq_m45, b_m45, eq_m46, b_m46, eq_m47, b_m47, eq_m48, b_m48,
-             one_of_45_46_47_48,
-             eq_m42, eq_m43, eq_m44,
-             lt_m49, lt_m53, h_15_44,
-             lt_m50, lt_m54, h_16_44,
-             lt_m51, lt_m55, h_17_44,
-             lt_m52, lt_m56, h_18_44,
-             eq_m57, eq_m58, eq_m59, eq_m60,
-             sll_00, sll_01, sll_02, sll_03, sll_04, sll_05, sll_06, sll_07, sll_08, sll_09, sll_10, sll_11, sll_12, sll_13, sll_14, sll_15,
-             sllw_00, sllw_01, sllw_02, sllw_03, sllw_04, sllw_05,
-             eq_m64 ⟩ := cstrs
-    have : Main[62] = 0 := by clear *- b_m62 b_m63; aesop
-    simp_all
-  . obtain ⟨ cpu, alu,
-             b_m36, b_m37, b_m38, b_m39, b_m40, b_m41,
-             diff_m25,
-             eq_m45, b_m45, eq_m46, b_m46, eq_m47, b_m47, eq_m48, b_m48,
-             one_of_45_46_47_48,
-             eq_m42, eq_m43, eq_m44,
-             lt_m49, lt_m53, h_15_44,
-             lt_m50, lt_m54, h_16_44,
-             lt_m51, lt_m55, h_17_44,
-             lt_m52, lt_m56, h_18_44,
-             eq_m57, eq_m58, eq_m59, eq_m60,
-             sllw_00, sllw_01, sllw_02, sllw_03, sllw_04, sllw_05,
-             eq_m62, eq_m64 ⟩ := cstrs
-    simp_all
-
-end slliw
-
 set_option maxHeartbeats 100000000 in
 lemma spec.slliw (h : is_slliw Main) :
   List.Forall SP1Constraint.toProp (constraints Main) →
     Main[25] < 32 ∧ Main[26] = 0 ∧ Main[27] = 0 ∧ Main[28] = 0 ∧
     Word.toBitVec64 #v[Main[32], Main[33], Main[34], Main[35]] = execute_RTYPEW_pure_w #v[Main[15], Main[16], Main[17], Main[18]] #v[Main[25], Main[26], Main[27], Main[28]] .SLLW
   := by sorry
-    -- intro cstrs; rw [allHold_constraints_iff_slliw h] at cstrs
+    -- intro cstrs; rw [allHold_constraints_iff] at cstrs
+    -- obtain ⟨ eq_sllw, eq_imm ⟩ := h
 
     -- set b0 := Main[15]
     -- set b1 := Main[16]
@@ -1156,6 +816,7 @@ lemma spec.slliw (h : is_slliw Main) :
     -- set c1 := Main[26]
     -- set c2 := Main[27]
     -- set c3 := Main[28]
+    -- set imm := Main[31]
     -- set a0 := Main[32]
     -- set a1 := Main[33]
     -- set a2 := Main[34]
@@ -1186,25 +847,31 @@ lemma spec.slliw (h : is_slliw Main) :
     -- set lr2 := Main[59]
     -- set lr3 := Main[60]
     -- set msb := Main[61]
+    -- set sll := Main[62]
+    -- set sllw := Main[63]
 
-    -- obtain ⟨ eq_m63, eq_m31 ⟩ := h
-    -- obtain ⟨ msb_cstrs, cpu_cstrs, alu_cstrs,
-    --          b_cb0, b_cb1, b_cb2, b_cb3, b_cb4, b_cb5,
-    --          diff,
-    --          eq_su160, b_su160, eq_su161, b_su161, eq_su162, b_su162, eq_su163, b_su163,
-    --          one_of_su16,
+    -- obtain ⟨ msb_a1, cpu, alu, one_of_ops,
+    --          b_sll, b_sllw,
+    --          b_cb0, b_cb1, b_cb2, b_cb3, b_cb4, b_cb5, diff,
+    --          h_su160, b_su160, h_su161, b_su161, h_su162, b_su162, h_su163, b_su163, one_of_su16s,
     --          eq_v01, eq_v012, eq_v0123,
-    --          lt_ll0, lt_hl0, h_b0_dec,
-    --          lt_ll1, lt_hl1, h_b1_dec,
-    --          lt_ll2, lt_hl2, h_b2_dec,
-    --          lt_ll3, lt_hl3, h_b3_dec,
+    --          lt_ll0, lt_lh0, h_b0_dec, lt_ll1, lt_lh1, h_b1_dec,
+    --          lt_ll2, lt_lh2, h_b2_dec, lt_ll3, lt_lh3, h_b3_dec,
     --          eq_lr0, eq_lr1, eq_lr2, eq_lr3,
-    --          sllw_00, sllw_01, sllw_02, sllw_03, sllw_04, sllw_05,
-    --          eq_m62, eq_m64 ⟩ := cstrs
-    -- clear cpu_cstrs
-    -- rw [ALUTypeReader.allHold_constraints_iff_is_real (by rfl)] at alu_cstrs
-    -- simp [Opcode.ofNat, Nat.ble, Nat.beq] at alu_cstrs
-    -- obtain ⟨ ⟨ h0, hc0, hc1, hc2, hc3 ⟩, h1, h2, h3, h4, h5, h6, h7, h8, h9, h10, h11, h12, h13, h14, is_U64_b, h15, eq_c0, eq_c1, eq_c2, eq_c3 ⟩ := alu_cstrs
+    --          nw_00, nw_01, nw_02, nw_03, nw_04, nw_05, nw_06, nw_07, nw_08, nw_09, nw_10, nw_11, nw_12, nw_13, nw_14, nw_15,
+    --          w_00, w_01, w_02, w_03, w_04, w_05,
+    --          eq_m64 ⟩ := cstrs
+
+    -- have eq_m63 : sll = 0 := by
+    --   clear *- b_sll b_sllw one_of_ops eq_sllw
+    --   simp_all; aesop
+
+    -- simp_all
+
+    -- clear cpu
+    -- rw [ALUTypeReader.allHold_constraints_iff_is_real (by rfl)] at alu
+    -- simp [Opcode.ofNat, Nat.ble, Nat.beq] at alu
+    -- obtain ⟨ ⟨ h0, hc0, hc1, hc2, hc3 ⟩, h1, h2, h3, h4, h5, h6, h7, h8, h9, h10, h11, h12, h13, h14, is_U64_b, h15, eq_c0, eq_c1, eq_c2, eq_c3 ⟩ := alu
     -- clear h0 h1 h2 h3 h4 h5 h6 h7 h8 h9 h10 h11 h12 h13 h14 h15
     -- rw [← eq_c0] at hc0 eq_c0; simp_all
 
@@ -1212,7 +879,7 @@ lemma spec.slliw (h : is_slliw Main) :
     -- simp_all
 
     -- have is_U32_b : HalfWord.isU32 #v[ b0, b1 ] := by apply HalfWord.isU32_of_cases <;> assumption
-    -- have is_U32_c : HalfWord.isU32 #v[ c0, 0 ] := by apply HalfWord.isU32_of_cases <;> simp <;> omega
+    -- have is_U32_c : HalfWord.isU32 #v[ c0, 0 ] := by apply HalfWord.isU32_of_cases <;> simp; omega
 
     -- have : ((Word.low32 #v[c0, 0, 0, 0]).toBitVec32.toNat % 32) = c0.val % 32 := by
     --   simp [Word.low32, HalfWord.toBitVec32_toNat is_U32_c, HalfWord.toNat]
@@ -1247,8 +914,9 @@ lemma spec.slliw (h : is_slliw Main) :
     -- have ⟨ _, _ ⟩ := HalfWord.lt_cases_of_isU32 h_isU32_a
 
     -- have h_a3 : a3 = if (HalfWord.toBitVec32 #v[a0, a1]).msb = true then 65535 else 0 := by
-    --   rw [← sllw_05, ← sllw_04]
-    --   have h_msb := U16MSBOperation.spec a1 { msb := msb } 1 (by assumption) msb_cstrs (by simp)
+    --   simp_all
+    --   rw [← w_04] at *
+    --   have h_msb := U16MSBOperation.spec a1 { msb := msb } 1 (by assumption) msb_a1 (by simp)
     --   simp at h_msb; rw [h_msb]
     --   trans (if HalfWord.isNegative #v[a0, a1] then 65535 else 0)
     --   . unfold HalfWord.isNegative; split_ifs <;> simp_all; omega
@@ -1275,5 +943,7 @@ lemma spec.slliw (h : is_slliw Main) :
     --       repeat rw [Nat.mod_eq_of_lt (b := 2013265921) (by omega)]
     --       omega
     --     }
+
+end slliw
 
 end ShiftLeft
