SP1Chips/ShiftLeftChip.lean
@@ -7,12 +7,14 @@ import SP1Chips.ShiftLeft.Constraints
 open LeanRV64IM.Functions
 open BitVec
 
+set_option maxHeartbeats 10000000
+
 namespace Sll
 
-open ShiftLeft
+open ShiftRight
 
 variable
-  (Main : Vector (Fin BB) 65)
+  (Main : Vector (Fin BB) 69)
   (s : SailState)
   (cstrs : (constraints Main).allHold)
   (h_is_sll : is_sll Main)
@@ -22,45 +24,9 @@ def spec_sll (rs2 rs1 rd : regidx) : SailM Unit := do
   _ ← execute_RTYPE rs2 rs1 rd rop.SLL
   pure ()
 
-def sp1_op_a : BitVec 5 :=
-  by
-    refine BitVec.ofNatLT Main[6] ?_
-    simp
-    show Main[6] < 32
-
-    rw [SP1ConstraintList.allHold, allHold_constraints_iff_sll h_is_sll] at cstrs
-    obtain ⟨ lt_op, cpu, alu, rest ⟩ := cstrs
-    simp [ALUTypeReader.constraints, SP1Constraint.toProp] at alu
-    simp_all [Opcode.ofNat, Nat.ble, Nat.beq]
-
-def sp1_op_b : BitVec 5 :=
-  by
-    refine BitVec.ofNatLT Main[14] ?_
-    simp
-    show Main[14] < 32
-
-    have alu_cstrs := by
-      simp [SP1ConstraintList.allHold, constraints, SP1Constraint.toProp] at cstrs
-      exact cstrs.2.2.1
-
-    rw [SP1ConstraintList.allHold, allHold_constraints_iff_sll h_is_sll] at cstrs
-    obtain ⟨ lt_op, cpu, alu, rest ⟩ := cstrs
-    simp [ALUTypeReader.constraints, SP1Constraint.toProp] at alu
-    simp_all [Opcode.ofNat, Nat.ble, Nat.beq]
-
-def sp1_op_c : BitVec 5 :=
-  by
-    refine BitVec.ofNatLT Main[21] ?_
-    simp
-    show Main[21] < 32
-
-    rw [SP1ConstraintList.allHold, allHold_constraints_iff_sll h_is_sll] at cstrs
-    obtain ⟨ lt_op, cpu, alu, rest ⟩ := cstrs
-    simp [ALUTypeReader.constraints, SP1Constraint.toProp] at alu
-    simp_all [Opcode.ofNat, Nat.ble, Nat.beq]
-
 def sp1_sll : SailM Unit := do
-  let op_a := sp1_op_a Main cstrs h_is_sll
+  let ⟨ sll, imm ⟩ := h_is_sll
+  let op_a := sp1_op_a Main cstrs (sll_real Main sll)
   -- TODO(gzgz): we can obtain this from the constraint compiler
   -- This comes from the Interaction.state in CPUState
   Sail.writeReg Register.nextPC (Word.toBitVec64 #v[Main[3], Main[4], Main[5], 0] + 4)
@@ -69,46 +35,29 @@ def sp1_sll : SailM Unit := do
 set_option maxHeartbeats 1000000 in
 theorem correct_sll
   (state_cstrs : (constraints Main).initialState s) :
-  let op_c := sp1_op_c Main cstrs h_is_sll
-  let op_b := sp1_op_b Main cstrs h_is_sll
-  let op_a := sp1_op_a Main cstrs h_is_sll
+  let ⟨ sll, imm ⟩ := h_is_sll
+  let op_c := sp1_op_c Main cstrs (sll_real Main sll) imm
+  let op_b := sp1_op_b Main cstrs (sll_real Main sll)
+  let op_a := sp1_op_a Main cstrs (sll_real Main sll)
   (spec_sll (.Regidx op_c) (.Regidx op_b) (.Regidx op_a)).run s = (sp1_sll Main cstrs h_is_sll).run s
   := by
-    -- Obtain and simplify state and pure constraints
-    simp [SP1ConstraintList.allHold] at cstrs; simp [is_sll] at h_is_sll
-    have spec := spec.sll h_is_sll cstrs
-    rw [allHold_constraints_iff_sll h_is_sll] at cstrs
-    obtain ⟨ eq_m62, eq_m31 ⟩ := h_is_sll
-    obtain ⟨ msb_cstrs, cpu_cstrs, alu_cstrs,
-             b_cb0, b_cb1, b_cb2, b_cb3, b_cb4, b_cb5,
-             diff,
-             eq_su160, b_su160, eq_su161, b_su161, eq_su162, b_su162, eq_su163, b_su163,
-             one_of_su16,
-             eq_v01, eq_v012, eq_v0123,
-             lt_ll0, lt_hl0, h_b0_dec,
-             lt_ll1, lt_hl1, h_b1_dec,
-             lt_ll2, lt_hl2, h_b2_dec,
-             lt_ll3, lt_hl3, h_b3_dec,
-             eq_lr0, eq_lr1, eq_lr2, eq_lr3,
-             sll_00, sll_01, sll_02, sll_03, sll_04, sll_05, sll_06, sll_07, sll_08, sll_09, sll_10, sll_11, sll_12, sll_13, sll_14, sll_15,
-             eq_m63, eq_m64 ⟩ := cstrs
-    rw [ALUTypeReader.allHold_constraints_iff_is_real (by rfl)] at alu_cstrs
-    simp [Opcode.ofNat, Nat.ble, Nat.beq] at alu_cstrs
-    obtain ⟨ h0, h1, h2, h3, h4, h5, h6, h7, h8, h9, h10, h11, h12, h13, h14, is_U64_b, ⟨ h15, h16, is_U64_c ⟩, h17 ⟩ := alu_cstrs
+    let ⟨ sll, imm ⟩ := h_is_sll
+    have ⟨ ha, hb, hc, is_U64_b, is_U64_c, h_imm, h_a0 ⟩ := bounds Main cstrs (sll_real Main sll)
+    have ⟨ sop1, sop2, sop3, sop4 ⟩ := single_op Main cstrs
+    simp_all
 
     simp [SP1ConstraintList.initialState, constraints, SP1Constraint.toStateProp, List.Forall, CPUState.constraints, ALUTypeReader.constraints] at state_cstrs
-    obtain ⟨throwaway, read_pc, trusted_instr_state, read_op_a, read_op_b, read_op_c⟩ := state_cstrs
-    clear throwaway; simp_all
-    simp [Opcode.ofNat, Nat.ble, Nat.beq] at *; simp_all
+    obtain ⟨thr1, thr2, thr3, read_pc, trusted_instr_state, read_op_a, read_op_b, read_op_c⟩ := state_cstrs
+    clear thr1 thr2 thr3 trusted_instr_state; simp_all
 
-    -- Now the monadic manipulation
     simp [spec_sll, sp1_sll, execute, execute_RTYPE']
     rw [Sail.run_readReg, read_pc]
     simp [sp1_op_a, sp1_op_b, sp1_op_c, read_op_b, read_op_c]
     by_cases h_is_op_a_0 : Main[6] = 0 <;> simp_all
-    . rw [← spec]; simp [Word.toBitVec64, Word.toNat]
+    . simp [Word.toBitVec64, Word.toNat]
     . rw [if_neg (by simpa [← BitVec.toNat_inj])]
       rw [if_neg (by simpa [← BitVec.toNat_inj])]
+      rw [spec.sll Main ⟨ sll, imm ⟩ cstrs]
       rw [exec_RTYPE_pure_bv_to_w _ _ _ (by omega) (by omega)]
       simp [Word.toBitVec64, Word.toNat]
       rfl
@@ -117,10 +66,10 @@ end Sll
 
 namespace Slli
 
-open ShiftLeft
+open ShiftRight
 
 variable
-  (Main : Vector (Fin BB) 65)
+  (Main : Vector (Fin BB) 69)
   (s : SailState)
   (cstrs : (constraints Main).allHold)
   (h_is_slli : is_slli Main)
@@ -130,96 +79,52 @@ def spec_slli (shamt : BitVec 6) (rs1 rd : regidx) : SailM Unit := do
   _ ← execute_SHIFTIOP shamt rs1 rd sop.SLLI
   pure ()
 
-def sp1_op_a : BitVec 5 :=
-  by
-    refine BitVec.ofNatLT Main[6] ?_
-    simp
-    show Main[6] < 32
-
-    rw [SP1ConstraintList.allHold, allHold_constraints_iff_slli h_is_slli] at cstrs
-    obtain ⟨ lt_op, cpu, alu, rest ⟩ := cstrs
-    simp [ALUTypeReader.constraints, SP1Constraint.toProp] at alu
-    simp_all [Opcode.ofNat, Nat.ble, Nat.beq]
-
-def sp1_op_b : BitVec 5 :=
-  by
-    refine BitVec.ofNatLT Main[14] ?_
-    simp
-    show Main[14] < 32
-
-    have alu_cstrs := by
-      simp [SP1ConstraintList.allHold, constraints, SP1Constraint.toProp] at cstrs
-      exact cstrs.2.2.1
-
-    rw [SP1ConstraintList.allHold, allHold_constraints_iff_slli h_is_slli] at cstrs
-    obtain ⟨ lt_op, cpu, alu, rest ⟩ := cstrs
-    simp [ALUTypeReader.constraints, SP1Constraint.toProp] at alu
-    simp_all [Opcode.ofNat, Nat.ble, Nat.beq]
-
-def sp1_op_c : BitVec 6 := BitVec.ofNat 6 Main[21]
-
 def sp1_slli : SailM Unit := do
-  let op_a := sp1_op_a Main cstrs h_is_slli
+  let ⟨ sll, imm ⟩ := h_is_slli
+  let op_a := sp1_op_a Main cstrs (sll_real Main sll)
   -- TODO(gzgz): we can obtain this from the constraint compiler
   -- This comes from the Interaction.state in CPUState
   Sail.writeReg Register.nextPC (Word.toBitVec64 #v[Main[3], Main[4], Main[5], 0] + 4)
   Sail.write_reg op_a (Word.toBitVec64 #v[Main[32], Main[33], Main[34], Main[35]])
 
 set_option maxHeartbeats 1000000 in
-theorem correct_sll
+theorem correct_slli
   (state_cstrs : (constraints Main).initialState s) :
-  let op_c := sp1_op_c Main
-  let op_b := sp1_op_b Main cstrs h_is_slli
-  let op_a := sp1_op_a Main cstrs h_is_slli
+  let ⟨ sll, imm ⟩ := h_is_slli
+  let op_c := sp1_op_c_imm Main cstrs (sll_real Main sll) imm (by tauto)
+  let op_b := sp1_op_b Main cstrs (sll_real Main sll)
+  let op_a := sp1_op_a Main cstrs (sll_real Main sll)
   (spec_slli op_c (.Regidx op_b) (.Regidx op_a)).run s = (sp1_slli Main cstrs h_is_slli).run s
   := by
-    -- Obtain and simplify state and pure constraints
-    simp [SP1ConstraintList.allHold] at cstrs; simp [is_sll] at h_is_slli
-    have spec := spec.slli h_is_slli cstrs
-    rw [allHold_constraints_iff_slli h_is_slli] at cstrs
-    obtain ⟨ eq_m62, eq_m31 ⟩ := h_is_slli
-    obtain ⟨ msb_cstrs, cpu_cstrs, alu_cstrs,
-             b_cb0, b_cb1, b_cb2, b_cb3, b_cb4, b_cb5,
-             diff,
-             eq_su160, b_su160, eq_su161, b_su161, eq_su162, b_su162, eq_su163, b_su163,
-             one_of_su16,
-             eq_v01, eq_v012, eq_v0123,
-             lt_ll0, lt_hl0, h_b0_dec,
-             lt_ll1, lt_hl1, h_b1_dec,
-             lt_ll2, lt_hl2, h_b2_dec,
-             lt_ll3, lt_hl3, h_b3_dec,
-             eq_lr0, eq_lr1, eq_lr2, eq_lr3,
-             sll_00, sll_01, sll_02, sll_03, sll_04, sll_05, sll_06, sll_07, sll_08, sll_09, sll_10, sll_11, sll_12, sll_13, sll_14, sll_15,
-             eq_m63, eq_m64 ⟩ := cstrs
-    rw [ALUTypeReader.allHold_constraints_iff_is_real (by rfl)] at alu_cstrs
-    simp [Opcode.ofNat, Nat.ble, Nat.beq] at alu_cstrs
-    obtain ⟨ ⟨ h0, hc0, hc1, hc2, hc3 ⟩, h1, h2, h3, h4, h5, h6, h7, h8, h9, h10, h11, h12, h13, h14, is_U64_b, h15, eq_c0, eq_c1, eq_c2, eq_c3 ⟩ := alu_cstrs
+    let ⟨ sll, imm ⟩ := h_is_slli
+    have ⟨ ha, hb, hc, is_U64_b, is_U64_c, h_imm, h_a0 ⟩ := bounds Main cstrs (sll_real Main sll)
+    have ⟨ sop1, sop2, sop3, sop4 ⟩ := single_op Main cstrs
+    simp_all
 
     simp [SP1ConstraintList.initialState, constraints, SP1Constraint.toStateProp, List.Forall, CPUState.constraints, ALUTypeReader.constraints] at state_cstrs
-    obtain ⟨throwaway, read_pc, trusted_instr_state, read_op_a, read_op_b, read_op_c⟩ := state_cstrs
-    clear throwaway; simp_all
-    simp [Opcode.ofNat, Nat.ble, Nat.beq] at *; simp_all
+    obtain ⟨thr1, thr2, thr3, read_pc, trusted_instr_state, read_op_a, read_op_b, read_op_c⟩ := state_cstrs
+    clear thr1 thr2 thr3 trusted_instr_state; simp_all
 
-    -- Now the monadic manipulation
     simp [spec_slli, sp1_slli, execute, execute_SHIFTIOP']
     rw [Sail.run_readReg, read_pc]
     simp [sp1_op_a, sp1_op_b, sp1_op_c, read_op_b]
     by_cases h_is_op_a_0 : Main[6] = 0 <;> simp_all
-    . rw [← spec]; simp [Word.toBitVec64, Word.toNat]
+    . simp [Word.toBitVec64, Word.toNat]
     . rw [if_neg (by simpa [← BitVec.toNat_inj])]
       rw [if_neg (by simpa [← BitVec.toNat_inj])]
+      rw [spec.slli Main ⟨ sll, imm ⟩ cstrs]
       rw [exec_SHIFTIOP_pure_bv_to_w _ _ _ is_U64_b]
-      simp [Word.toBitVec64, Word.toNat]
+      simp_all [Word.toBitVec64, Word.toNat]
       rfl
 
 end Slli
 
 namespace Sllw
 
-open ShiftLeft
+open ShiftRight
 
 variable
-  (Main : Vector (Fin BB) 65)
+  (Main : Vector (Fin BB) 69)
   (s : SailState)
   (cstrs : (constraints Main).allHold)
   (h_is_sllw : is_sllw Main)
@@ -229,93 +134,40 @@ def spec_sllw (rs2 rs1 rd : regidx) : SailM Unit := do
   _ ← execute_RTYPEW rs2 rs1 rd ropw.SLLW
   pure ()
 
-def sp1_op_a : BitVec 5 :=
-  by
-    refine BitVec.ofNatLT Main[6] ?_
-    simp
-    show Main[6] < 32
-
-    rw [SP1ConstraintList.allHold, allHold_constraints_iff_sllw h_is_sllw] at cstrs
-    obtain ⟨ lt_op, cpu, alu, rest ⟩ := cstrs
-    simp [ALUTypeReader.constraints, SP1Constraint.toProp] at alu
-    simp_all [Opcode.ofNat, Nat.ble, Nat.beq]
-
-def sp1_op_b : BitVec 5 :=
-  by
-    refine BitVec.ofNatLT Main[14] ?_
-    simp
-    show Main[14] < 32
-
-    have alu_cstrs := by
-      simp [SP1ConstraintList.allHold, constraints, SP1Constraint.toProp] at cstrs
-      exact cstrs.2.2.1
-
-    rw [SP1ConstraintList.allHold, allHold_constraints_iff_sllw h_is_sllw] at cstrs
-    obtain ⟨ lt_op, cpu, alu, rest ⟩ := cstrs
-    simp [ALUTypeReader.constraints, SP1Constraint.toProp] at alu
-    simp_all [Opcode.ofNat, Nat.ble, Nat.beq]
-
-def sp1_op_c : BitVec 5 :=
-  by
-    refine BitVec.ofNatLT Main[21] ?_
-    simp
-    show Main[21] < 32
-
-    rw [SP1ConstraintList.allHold, allHold_constraints_iff_sllw h_is_sllw] at cstrs
-    obtain ⟨ lt_op, cpu, alu, rest ⟩ := cstrs
-    simp [ALUTypeReader.constraints, SP1Constraint.toProp] at alu
-    simp_all [Opcode.ofNat, Nat.ble, Nat.beq]
-
 def sp1_sllw : SailM Unit := do
-  let op_a := sp1_op_a Main cstrs h_is_sllw
+  let ⟨ sllw, imm ⟩ := h_is_sllw
+  let op_a := sp1_op_a Main cstrs (sllw_real Main sllw)
   -- TODO(gzgz): we can obtain this from the constraint compiler
   -- This comes from the Interaction.state in CPUState
   Sail.writeReg Register.nextPC (Word.toBitVec64 #v[Main[3], Main[4], Main[5], 0] + 4)
   Sail.write_reg op_a (Word.toBitVec64 #v[Main[32], Main[33], Main[34], Main[35]])
 
 set_option maxHeartbeats 1000000 in
-theorem correct_sll
+theorem correct_sllw
   (state_cstrs : (constraints Main).initialState s) :
-  let op_c := sp1_op_c Main cstrs h_is_sllw
-  let op_b := sp1_op_b Main cstrs h_is_sllw
-  let op_a := sp1_op_a Main cstrs h_is_sllw
+  let ⟨ sllw, imm ⟩ := h_is_sllw
+  let op_c := sp1_op_c Main cstrs (sllw_real Main sllw) imm
+  let op_b := sp1_op_b Main cstrs (sllw_real Main sllw)
+  let op_a := sp1_op_a Main cstrs (sllw_real Main sllw)
   (spec_sllw (.Regidx op_c) (.Regidx op_b) (.Regidx op_a)).run s = (sp1_sllw Main cstrs h_is_sllw).run s
   := by
-    -- Obtain and simplify state and pure constraints
-    simp [SP1ConstraintList.allHold] at cstrs; simp [is_sll] at h_is_sllw
-    have spec := spec.sllw h_is_sllw cstrs
-    rw [allHold_constraints_iff_sllw h_is_sllw] at cstrs
-    obtain ⟨ eq_m63, eq_m31 ⟩ := h_is_sllw
-    obtain ⟨ msb_cstrs, cpu_cstrs, alu_cstrs,
-             b_cb0, b_cb1, b_cb2, b_cb3, b_cb4, b_cb5,
-             diff,
-             eq_su160, b_su160, eq_su161, b_su161, eq_su162, b_su162, eq_su163, b_su163,
-             one_of_su16,
-             eq_v01, eq_v012, eq_v0123,
-             lt_ll0, lt_hl0, h_b0_dec,
-             lt_ll1, lt_hl1, h_b1_dec,
-             lt_ll2, lt_hl2, h_b2_dec,
-             lt_ll3, lt_hl3, h_b3_dec,
-             eq_lr0, eq_lr1, eq_lr2, eq_lr3,
-             sllw_00, sllw_01, sllw_02, sllw_03, sllw_04, sllw_05,
-             eq_m62, eq_m64 ⟩ := cstrs
-    rw [ALUTypeReader.allHold_constraints_iff_is_real (by rfl)] at alu_cstrs
-    simp [Opcode.ofNat, Nat.ble, Nat.beq] at alu_cstrs
-    obtain ⟨ h0, h1, h2, h3, h4, h5, h6, h7, h8, h9, h10, h11, h12, h13, h14, is_U64_b, ⟨ h15, h16, is_U64_c ⟩, h17 ⟩ := alu_cstrs
+    let ⟨ sllw, imm ⟩ := h_is_sllw
+    have ⟨ ha, hb, hc, is_U64_b, is_U64_c, h_imm, h_a0 ⟩ := bounds Main cstrs (sllw_real Main sllw)
+    have ⟨ sop1, sop2, sop3, sop4 ⟩ := single_op Main cstrs
+    simp_all
 
     simp [SP1ConstraintList.initialState, constraints, SP1Constraint.toStateProp, List.Forall, CPUState.constraints, ALUTypeReader.constraints] at state_cstrs
-    obtain ⟨throwaway, read_pc, trusted_instr_state, read_op_a, read_op_b, read_op_c⟩ := state_cstrs
-    clear throwaway; simp_all
-    simp [Opcode.ofNat, Nat.ble, Nat.beq] at *; simp_all
+    obtain ⟨thr1, thr2, thr3, read_pc, trusted_instr_state, read_op_a, read_op_b, read_op_c⟩ := state_cstrs
+    clear thr1 thr2 thr3 trusted_instr_state; simp_all
 
-    -- Now the monadic manipulation
     simp [spec_sllw, sp1_sllw, execute, execute_RTYPEW']
     rw [Sail.run_readReg, read_pc]
     simp [sp1_op_a, sp1_op_b, sp1_op_c, read_op_b, read_op_c]
     by_cases h_is_op_a_0 : Main[6] = 0 <;> simp_all
-    . rw [← spec]; simp [Word.toBitVec64, Word.toNat]
+    . simp [Word.toBitVec64, Word.toNat]
     . rw [if_neg (by simpa [← BitVec.toNat_inj])]
       rw [if_neg (by simpa [← BitVec.toNat_inj])]
+      rw [spec.sllw Main ⟨ sllw, imm ⟩ cstrs]
       rw [exec_RTYPEW_pure_bv_to_w _ _ _ (by omega) (by omega)]
       simp [Word.toBitVec64, Word.toNat]
       rfl
@@ -324,10 +176,10 @@ end Sllw
 
 namespace Slliw
 
-open ShiftLeft
+open ShiftRight
 
 variable
-  (Main : Vector (Fin BB) 65)
+  (Main : Vector (Fin BB) 69)
   (s : SailState)
   (cstrs : (constraints Main).allHold)
   (h_is_slliw : is_slliw Main)
@@ -337,86 +189,42 @@ def spec_slliw (shamt : BitVec 6) (rs1 rd : regidx) : SailM Unit := do
   _ ← execute_SHIFTIWOP shamt rs1 rd sopw.SLLIW
   pure ()
 
-def sp1_op_a : BitVec 5 :=
-  by
-    refine BitVec.ofNatLT Main[6] ?_
-    simp
-    show Main[6] < 32
-
-    rw [SP1ConstraintList.allHold, allHold_constraints_iff_slliw h_is_slliw] at cstrs
-    obtain ⟨ lt_op, cpu, alu, rest ⟩ := cstrs
-    simp [ALUTypeReader.constraints, SP1Constraint.toProp] at alu
-    simp_all [Opcode.ofNat, Nat.ble, Nat.beq]
-
-def sp1_op_b : BitVec 5 :=
-  by
-    refine BitVec.ofNatLT Main[14] ?_
-    simp
-    show Main[14] < 32
-
-    have alu_cstrs := by
-      simp [SP1ConstraintList.allHold, constraints, SP1Constraint.toProp] at cstrs
-      exact cstrs.2.2.1
-
-    rw [SP1ConstraintList.allHold, allHold_constraints_iff_slliw h_is_slliw] at cstrs
-    obtain ⟨ lt_op, cpu, alu, rest ⟩ := cstrs
-    simp [ALUTypeReader.constraints, SP1Constraint.toProp] at alu
-    simp_all [Opcode.ofNat, Nat.ble, Nat.beq]
-
-def sp1_op_c : BitVec 6 := BitVec.ofNat 6 Main[21]
-
 def sp1_slliw : SailM Unit := do
-  let op_a := sp1_op_a Main cstrs h_is_slliw
+  let ⟨ sllw, imm ⟩ := h_is_slliw
+  let op_a := sp1_op_a Main cstrs (sllw_real Main sllw)
   -- TODO(gzgz): we can obtain this from the constraint compiler
   -- This comes from the Interaction.state in CPUState
   Sail.writeReg Register.nextPC (Word.toBitVec64 #v[Main[3], Main[4], Main[5], 0] + 4)
   Sail.write_reg op_a (Word.toBitVec64 #v[Main[32], Main[33], Main[34], Main[35]])
 
 set_option maxHeartbeats 1000000 in
-theorem correct_sll
+theorem correct_slliw
   (state_cstrs : (constraints Main).initialState s) :
-  let op_c := sp1_op_c Main
-  let op_b := sp1_op_b Main cstrs h_is_slliw
-  let op_a := sp1_op_a Main cstrs h_is_slliw
+  let ⟨ sllw, imm ⟩ := h_is_slliw
+  let op_c := sp1_op_c_imm_w Main cstrs (sllw_real Main sllw) imm (by tauto)
+  let op_b := sp1_op_b Main cstrs (sllw_real Main sllw)
+  let op_a := sp1_op_a Main cstrs (sllw_real Main sllw)
   (spec_slliw op_c (.Regidx op_b) (.Regidx op_a)).run s = (sp1_slliw Main cstrs h_is_slliw).run s
   := by
-    -- Obtain and simplify state and pure constraints
-    simp [SP1ConstraintList.allHold] at cstrs; simp [is_sll] at h_is_slliw
-    have ⟨ m25, m26, m27, m28, spec ⟩ := spec.slliw h_is_slliw cstrs
-    rw [allHold_constraints_iff_slliw h_is_slliw] at cstrs
-    obtain ⟨ eq_m63, eq_m31 ⟩ := h_is_slliw
-    obtain ⟨ msb_cstrs, cpu_cstrs, alu_cstrs,
-             b_cb0, b_cb1, b_cb2, b_cb3, b_cb4, b_cb5,
-             diff,
-             eq_su160, b_su160, eq_su161, b_su161, eq_su162, b_su162, eq_su163, b_su163,
-             one_of_su16,
-             eq_v01, eq_v012, eq_v0123,
-             lt_ll0, lt_hl0, h_b0_dec,
-             lt_ll1, lt_hl1, h_b1_dec,
-             lt_ll2, lt_hl2, h_b2_dec,
-             lt_ll3, lt_hl3, h_b3_dec,
-             eq_lr0, eq_lr1, eq_lr2, eq_lr3,
-             sllw_00, sllw_01, sllw_02, sllw_03, sllw_04, sllw_05,
-             eq_m62, eq_m64 ⟩ := cstrs
-    rw [ALUTypeReader.allHold_constraints_iff_is_real (by rfl)] at alu_cstrs
-    simp [Opcode.ofNat, Nat.ble, Nat.beq] at alu_cstrs
-    obtain ⟨ ⟨ h0, hc0, hc1, hc2, hc3 ⟩, h1, h2, h3, h4, h5, h6, h7, h8, h9, h10, h11, h12, h13, h14, is_U64_b, h15, eq_c0, eq_c1, eq_c2, eq_c3 ⟩ := alu_cstrs
+    let ⟨ sllw, imm ⟩ := h_is_slliw
+    have ⟨ ha, hb, hc, is_U64_b, is_U64_c, h_imm, h_a0 ⟩ := bounds Main cstrs (sllw_real Main sllw)
+    have ⟨ sop1, sop2, sop3, sop4 ⟩ := single_op Main cstrs
+    simp_all
 
     simp [SP1ConstraintList.initialState, constraints, SP1Constraint.toStateProp, List.Forall, CPUState.constraints, ALUTypeReader.constraints] at state_cstrs
-    obtain ⟨throwaway, read_pc, trusted_instr_state, read_op_a, read_op_b, read_op_c⟩ := state_cstrs
-    clear throwaway; simp_all
-    simp [Opcode.ofNat, Nat.ble, Nat.beq] at *; simp_all
+    obtain ⟨thr1, thr2, thr3, read_pc, trusted_instr_state, read_op_a, read_op_b, read_op_c⟩ := state_cstrs
+    clear thr1 thr2 thr3 trusted_instr_state; simp_all
 
-    -- Now the monadic manipulation
     simp [spec_slliw, sp1_slliw, execute, execute_SHIFTIWOP']
     rw [Sail.run_readReg, read_pc]
     simp [sp1_op_a, sp1_op_b, sp1_op_c, read_op_b]
     by_cases h_is_op_a_0 : Main[6] = 0 <;> simp_all
-    . rw [← spec]; simp [Word.toBitVec64, Word.toNat]
+    . simp [Word.toBitVec64, Word.toNat]
     . rw [if_neg (by simpa [← BitVec.toNat_inj])]
       rw [if_neg (by simpa [← BitVec.toNat_inj])]
+      rw [spec.slliw Main ⟨ sllw, imm ⟩ cstrs]
       rw [exec_SHIFTIWOP_pure_bv_to_w _ _ _ is_U64_b]
-      simp [Word.toBitVec64, Word.toNat]
-      congr; simpa
+      simp_all [Word.toBitVec64, Word.toNat]
+      rfl
 
 end Slliw
